\documentclass[12pt]{book}
\usepackage{diffyqssetupUB}

\begin{document}

%extra exercises {Introduction to differential equations}


\begin{exercise}
%http://math.buffalo.edu/306/2019_06_13/001 

Verify that the function(s) solve the following differential equations (DEs):
\begin{enumerate}[a)]
    \item $y' = -5y\ ;\ y = 3e^{-5x}$
    \item $y' = \cos(3x)\ ;\ y = \frac{1}{3} \sin(3x) +7$
    \item $y' = 2y\ ;\ y = ce^{2x}\ , \text{where c is any real number.} $
    \item $y''+y'-6y = 0\ ;\ y_1 = e^{2x},\ y_2 = e^{-3x}$
    \item $y''+16y = 0\ ;\ y_1 = \cos(4x),\ y_2 = \sin(4x)$
\end{enumerate}
{\color{teal}BH all ok}
\end{exercise}

\begin{exercise}
%http://math.buffalo.edu/306/2019_06_13/002 

Substitute $y = e^{rx}$ into the following DEs, solve for $r$, then write the
{\color{red} general solution for the DE}
{\color{blue} general linear combination of the solution(s) of the form $e^{rx}$:}
{\color{teal}JR: Students are not told until Ch 2 that the general solution of an nth order homogeneous linear equation is the general linear combination of n linearly independent solutions.}
{\color{teal}BH rephrased question to
ask for general linear combination
rather then general solution}
\begin{enumerate}[a)]
    \item $7y'+5y = 0$
    \item $2y'' + 7y' -4y = 0$
    \item $y''-3y'-10y=0$
    \item $3y''-7y'-6y = 0$
    \item $4y''+3y'-y = 0$
\end{enumerate}

\end{exercise}
\exsol{%
\begin{enumerate}[a)]
    \item {\color{blue}$y = c e^{-\frac{5}{7}x}$}
    \item {\color{blue}$y = c_1 e^{\frac{1}{2}x}+ c_2 e^{-4x}$}
    \item {\color{blue}$y= c_1 e^{5x}+ c_2 e^{-2x}$}
    \item {\color{blue}$y = c_1 e^{-\frac{2}{3}x}+ c_2 e^{3x}$}
    \item {\color{blue}$y = c_1 e^{-x}+ c_2 e^{\frac{1}{4}x}$}
\end{enumerate}
{\color{teal}BH all ok}
}

\begin{exercise}
%http://math.buffalo.edu/306/2019_06_13/003
Verify that $y = y(x)$ solves the DE. Then find the constant $C$ which satisfies the given initial condition.
\begin{enumerate}[a)]
    \item $3y' = 2y,\ y(0)= 5\ ;\ y= Ce^{\frac{2}{3}x}$
    \item 
    {\color{blue}
    $y' = (3x^2 +1)y ,\ y(1)=1 \ ;\ y = C e^{x^{3}+x}$
    }
    {\color{teal}BH corrected missing factor $y$ in ode, JJ ok}
    \item $y' = 8x^3(y^2 +1),\ y(0)=1 \ ;\ y = \tan(2x^4 + C)$
    \item $y'+2y = 6,\ y(0)=-5 \ ;\ y = 3+ C e^{-2x}$
\end{enumerate}
\end{exercise}
\exsol{%
\begin{enumerate}[a)]
    \item $C = 5$
    \item $C = e^{-2}$
    \item $C = \frac{\pi}{4}$
    \item $C = -8$
\end{enumerate}
{\color{teal}BH all ok}
}
\printanswers
\end{document}









